upd

examples/airlock.v
@@ -23,16 +23,13 @@ Inductive door : Type := left | right.
 
 HB.instance Definition _ := gen_eqMixin door.
 
-Inductive DOORS : interface :=
+Inductive DOORS : effect :=
 | IsOpen : door -> DOORS bool
 | Toggle : door -> DOORS unit.
 
 Generalizable All Variables.
 
-Arguments request {_ } _ _ _.
-
-(* TODO: meaningful name section *)
-Section a.
+Section airlock_s.
 
 Import FreerFuns.
 
@@ -56,7 +53,7 @@ Definition close_door `{Provide ix DOORS} {im : freerMonad ix}
 
 (** ** Controller *)
 
-Inductive CONTROLLER : interface :=
+Inductive CONTROLLER : effect :=
 | Tick : CONTROLLER unit
 | RequestOpen (d : door) : CONTROLLER unit.
 
@@ -79,7 +76,7 @@ Proof. by []. Qed.
 Definition controller `{Provide ix DOORS, Provide ix (STORE nat)}
     {im : freerMonad ix} : component (im:=im) CONTROLLER ix
   (* .
-  move=>X; case=>[|d].
+  move=> X; case=> [|d].
   - apply/bind=>[|cpt].
     + apply/iget.
     + apply/when.
@@ -105,9 +102,9 @@ Definition controller `{Provide ix DOORS, Provide ix (STORE nat)}
         close_door right >>
         iput 0
     | RequestOpen d =>
-        close_door (co d) >>
-        open_door d >>
-        iput 0
+      close_door (co d) >>
+      open_door d >>
+      iput 0
     end.
 
 (** * Verifying the Airlock Controller *)
@@ -126,20 +123,16 @@ Definition sel (d : door) : Ω -> bool :=
 
 Definition tog (d : door) (ω : Ω) : Ω :=
   match d with
-  | left => (negb (fst ω), snd ω)
-  | right => (fst ω, negb (snd ω))
+  | left => (~~ (fst ω), snd ω)
+  | right => (fst ω, ~~ (snd ω))
   end.
 
 Lemma tog_equ_1 (d : door) (ω : Ω)
-  : sel d (tog d ω) = negb (sel d ω).
-
-Proof.
-  by case:d.
-Qed.
+  : sel d (tog d ω) = ~~ (sel d ω).
+Proof. by case: d. Qed.
 
 Lemma tog_equ_2 (d : door) (ω : Ω)
   : sel (co d) (tog d ω) = sel (co d) ω.
-
 Proof. by case: d. Qed.
 
 (** From now on, we will reason about [tog] using [tog_equ_1] and [tog_equ_2].
@@ -162,38 +155,26 @@ Definition step (ω : Ω) (a : Type) (e : DOORS a) (x : a) :=
 (** *** Requirements *)
 
 Inductive doors_o_caller : Ω -> forall (a : Type), DOORS a -> Prop :=
-
 (** - Given the door [d] of o system [ω], it is always possible to ask for the
       state of [d]. *)
-
 | req_is_open (d : door) (ω : Ω)
   : doors_o_caller ω bool (IsOpen d)
-
 (** - Given the door [d] of o system [ω], if [d] is closed, then the second door
       [co d] has to be closed too for a request to toggle [d] to be valid. *)
-
 | req_toggle (d : door) (ω : Ω) (H : sel d ω = false -> sel (co d) ω = false)
   : doors_o_caller ω unit (Toggle d).
-
-Hint Constructors doors_o_caller : airlock.
 
 (** *** Promises *)
 
 Inductive doors_o_callee : Ω -> forall (a : Type), DOORS a -> a -> Prop :=
-
 (** - When a system in a state [ω] reports the state of the door [d], it shall
       reflect the true state of [d]. *)
-
 | doors_o_callee_is_open (d : door) (ω : Ω) (x : bool) (equ : sel d ω = x)
   : doors_o_callee ω bool (IsOpen d) x
-
 (** - There is no particular requirement on the result [x] of a request for
       [ω] to close the door [d]. *)
-
 | doors_o_callee_toggle (d : door) (ω : Ω) (x : unit)
   : doors_o_callee ω unit (Toggle d) x.
-
- Hint Constructors doors_o_callee : airlock.
 
 Definition doors_contract : contract DOORS Ω :=
   make_contract step doors_o_caller doors_o_callee.
@@ -202,159 +183,112 @@ Definition doors_contract : contract DOORS Ω :=
 
 Lemma doors_is_open_calleeE (ω : Ω) (d : door) (x : bool) :
   doors_o_callee ω bool (IsOpen d) x -> sel d ω = x.
-Proof.
-(* case: x; case. *)
-
-move=> reported.
-case x; inversion reported; ssubst=>//=.
-Admitted.
+Proof. by case: x=> postc; inversion postc; ssubst. Qed.
 
 Lemma doors_toggle_callerE (ω : Ω) (d : door) :
   doors_o_caller ω unit (Toggle d) ->
   sel d ω = false -> sel (co d) ω = false.
 Proof.
-move=> allowed.
-by inversion allowed as [d' ω' | d' ω' safe]; subst.
+by move=> allowed; inversion allowed as [d' ω' | d' ω' safe]; subst.
 Qed.
 
 (** Closing a door [d] in any system [ω] is always a respectful operation. *)
 
 Lemma close_door_respectful `{Provide ix DOORS} (ω : Ω) (d : door) :
-  pre (to_hoare
-         (im:=Freer.Monad_acto__canonical__Impure_MonadFreer ix)
-         doors_contract (close_door d)) ω.
-
+  pre (to_hoare (im:=freer ix) doors_contract (close_door d)) ω.
 Proof.
 rewrite /close_door /is_open.
+apply/to_hoare_impure_preI=> [|opened].
+- by rewrite /gen_caller_obligation proj_inj_p_equ /=; exact: req_is_open.
+rewrite /gen_callee_obligation /gen_witness_update !proj_inj_p_equ /=.
+move=> isopen_post.
+have isopen_post_equ := doors_is_open_calleeE ω d opened isopen_post.
+move: isopen_post isopen_post_equ=> _.
+rewrite /when /toggle; case: opened=> isopen_post_equ; last first.
+- exact: to_hoare_skip_preI.
+Check to_hoare_skip_preI.
+apply/to_hoare_impure_preI.
+- rewrite /gen_caller_obligation proj_inj_p_equ /=; apply: req_toggle.
+  by rewrite isopen_post_equ.
+- by move=> *; exact: to_hoare_skip_preI.
+Qed.
+
+Lemma open_door_respectful `{Provide ix DOORS} (ω : Ω)
+    (d : door) (safe : sel (co d) ω = false) :
+  pre (to_hoare (im:=freer ix) doors_contract (open_door (ix := ix) d)) ω.
+Proof.
+rewrite /open_door /is_open.
 apply/to_hoare_impure_preI.
 - rewrite /gen_caller_obligation proj_inj_p_equ /=.
   exact: req_is_open.
 move=> opened.
 rewrite /gen_callee_obligation /gen_witness_update !proj_inj_p_equ /=.
-move=> reported.
-have reported_equ := doors_is_open_calleeE ω d opened reported.
-clear reported.
-case: opened reported_equ => reported_equ.
-- rewrite /when /toggle.
-  apply/to_hoare_impure_preI.
-  + rewrite /gen_caller_obligation proj_inj_p_equ /=.
-    apply: req_toggle => closed.
-    by rewrite reported_equ in closed.
-  + move=> toggle_result _.
-    exact: to_hoare_local_preI.
-rewrite /when.
-exact: to_hoare_local_preI.
-
-  (* This leaves us with one goal to prove:
-
-       [sel d ω = false -> sel (co d) ω = false]
-
-     Yet, thanks to our call to [IsOpen d], we can predict that
-
-       [sel d ω = true] *)
-
-Qed.
-
- Hint Resolve close_door_respectful : airlock.
-
-Lemma open_door_respectful `{Provide ix DOORS} (ω : Ω)
-    (d : door) (safe : sel (co d) ω = false) :
-  pre (to_hoare
-         (im:=Freer.Monad_acto__canonical__Impure_MonadFreer ix)
-         doors_contract (open_door (ix := ix) d)) ω.
-
-Proof.
-rewrite /open_door /is_open.
-apply/to_hoare_impure_preI.
-  - rewrite /gen_caller_obligation proj_inj_p_equ /=.
-    exact: req_is_open.
-move=> opened.
-rewrite /gen_callee_obligation /gen_witness_update !proj_inj_p_equ /=.
-move=> reported.
-have reported_equ := doors_is_open_calleeE ω d opened reported.
-clear reported.
-case: opened reported_equ => reported_equ.
-  - rewrite /when.
-    exact: to_hoare_local_preI.
+move=> isopen_post.
+have isopen_post_equ := doors_is_open_calleeE ω d opened isopen_post.
+move: isopen_post=>_.
+case: opened isopen_post_equ => isopen_post_equ.
+- rewrite /when.
+  exact: to_hoare_skip_preI.
 rewrite /when /toggle.
 apply/to_hoare_impure_preI.
-  - rewrite /gen_caller_obligation proj_inj_p_equ /=.
-    by apply: req_toggle.
+- rewrite /gen_caller_obligation proj_inj_p_equ /=.
+  by apply: req_toggle.
 move=> toggle_result _.
-exact: to_hoare_local_preI.
+exact: to_hoare_skip_preI.
 Qed.
-
- Hint Resolve open_door_respectful : airlock.
 
 Lemma store_request_preI `{StrictProvide2 ix DOORS (STORE nat)}
     `(e : STORE nat a) (ω : Ω) :
-  pre (to_hoare
-         (im:=Freer.Monad_acto__canonical__Impure_MonadFreer ix)
-         doors_contract
-         (@request ix
-           (Freer.Monad_acto__canonical__Impure_MonadFreer ix)
-           a (inj_p e))) ω.
+  pre (to_hoare (im:=freer ix)
+         doors_contract (trigger (inj_p e))) ω.
 Proof.
-by apply/to_hoare_request_preE; rewrite /gen_caller_obligation distinguish.
+by apply/to_hoare_request_preE; rewrite /gen_caller_obligation /= distinguish.
 Qed.
 
 Lemma doors_is_open_postE `{Provide ix DOORS} (ω : Ω) (d : door)
     (opened : bool) (ω' : Ω) :
   post (to_hoare
-          (im:=Freer.Monad_acto__canonical__Impure_MonadFreer ix)
+          (im:=freer ix)
           doors_contract (is_open d)) ω opened ω' ->
   sel d ω = opened /\ ω' = ω.
 Proof.
 rewrite /is_open.
-move=> /to_hoare_request_postE [reported witness].
-rewrite /gen_callee_obligation proj_inj_p_equ /= in reported.
+move=> /to_hoare_request_postE [isopen_post witness].
+rewrite /gen_callee_obligation proj_inj_p_equ /= in isopen_post.
 rewrite /gen_witness_update proj_inj_p_equ /= in witness.
 split.
-- exact: doors_is_open_calleeE ω d opened reported.
+- exact: doors_is_open_calleeE ω d opened isopen_post.
 - exact: witness.
 Qed.
 
 Lemma doors_toggle_postE `{Provide ix DOORS} (ω : Ω) (d : door)
     (result : unit) (ω' : Ω) :
   post (to_hoare
-          (im:=Freer.Monad_acto__canonical__Impure_MonadFreer ix)
+          (im:=freer ix)
           doors_contract (toggle d)) ω result ω' ->
   ω' = tog d ω.
 Proof.
-rewrite /toggle.
-move=> /to_hoare_request_postE. move=> [_ witness].
-by rewrite /gen_witness_update proj_inj_p_equ /= in witness.
+rewrite /toggle to_hoare_request_postE /gen_witness_update proj_inj_p_equ /=.
+by move=> [_ ->].
 Qed.
 
 Lemma close_door_run `{Provide ix DOORS} (ω : Ω) (d : door)
     (ω' : Ω) (x : unit)
     (run : post (to_hoare
-      (im:=Freer.Monad_acto__canonical__Impure_MonadFreer ix)
+      (im:=freer ix)
       doors_contract (close_door d)) ω x ω') :
   sel d ω' = false.
 Proof.
-rewrite /close_door in run.
-move: run => /to_hoare_bind_postE [open [ω1 [opened tail]]].
-move: opened => /doors_is_open_postE [reported witness].
-subst ω1.
-case is_open_equ: (sel d ω) reported tail => reported tail.
-- cbn in tail.
-  rewrite -reported in tail.
-  cbn in tail.
-  move: tail => /to_hoare_bind_postE
-    [toggle_result [ω2 [toggle_run done]]].
-  move: toggle_run => /doors_toggle_postE toggle_witness.
-  move: done => /to_hoare_local_postE [_ local_witness].
-  subst ω2; subst ω'.
-  by rewrite tog_equ_1 is_open_equ.
-- rewrite -reported in tail.
-  cbn in tail.
-  move: tail => /to_hoare_local_postE [_ witness].
-  subst ω'.
-  exact: is_open_equ.
+move: run.
+rewrite /close_door to_hoare_bind_postE.
+move=>[opened [? [+ +]]]=> /doors_is_open_postE [+ ->]/=.
+case is_open_equ: (sel d ω)=> <-; last first.
+- by rewrite to_hoare_local_postE=> -[_ <-].
+rewrite to_hoare_bind_postE=> -[a [w' [/doors_toggle_postE +]]]=> -> /to_hoare_local_postE [_ <-].
+by rewrite tog_equ_1 is_open_equ.
 Qed.
 
- Hint Resolve close_door_run : airlock.
+Hint Resolve close_door_run : airlock.
 
 #[local] Opaque close_door.
 #[local] Opaque open_door.
@@ -363,15 +297,14 @@ Qed.
 Remark one_door_safe_all_doors_safe (ω : Ω) (d : door)
     (safe : sel d ω = false \/ sel (co d) ω = false)
   : forall (d' : door), sel d' ω = false \/ sel (co d') ω = false.
-
 Proof.
-  intros d'.
-  destruct d; destruct d'; auto.
-  + cbn -[sel].
-    now rewrite or_comm.
-  + cbn -[sel].
-    fold (co right).
-    now rewrite or_comm.
+intros d'.
+destruct d; destruct d'; auto.
+- cbn -[sel].
+  now rewrite or_comm.
+- cbn -[sel].
+  fold (co right).
+  now rewrite or_comm.
 Qed.
 
 (** The objective of this lemma is to prove that, if either the right door or
@@ -382,50 +315,50 @@ Qed.
 Definition doors_safe (ω : Ω) :=
   sel left ω = false \/ sel right ω = false.
 
-Lemma doors_request_preserves_safe {ix a}  {mp : MayProvide ix DOORS}
+Lemma doors_request_preserves_safe {ix a} {mp : MayProvide ix DOORS}
     {provided : @Provide ix DOORS mp}
     (e : ix a) (ω : Ω) (x : a) (ω' : Ω) :
   pre (to_hoare
-         (im:=Freer.Monad_acto__canonical__Impure_MonadFreer ix)
+         (im:=freer ix)
          doors_contract (trigger e)) ω ->
   post (to_hoare
-          (im:=Freer.Monad_acto__canonical__Impure_MonadFreer ix)
+          (im:=freer ix)
           doors_contract (trigger e)) ω x ω' ->
   doors_safe ω ->
   doors_safe ω'.
 Proof.
-  case projected: (@proj_p ix DOORS mp a e) => [door_request |];
-  rewrite to_hoare_request_preE to_hoare_request_postE;
-  rewrite /gen_caller_obligation /gen_callee_obligation /gen_witness_update projected //=; last first.
-  - by move=> _ [_ ->].
+case projected: (@proj_p ix DOORS mp a e) => [door_request |];
+rewrite to_hoare_request_preE to_hoare_request_postE;
+rewrite /gen_caller_obligation /gen_callee_obligation /gen_witness_update
+  projected //=; last first.
+- by move=> _ [_ ->].
 
-  move: door_request projected x=> + _.
+move: door_request projected x=> + _.
 
-  case=> d x prec postc safe; apply one_door_safe_all_doors_safe with (d := d);
-    apply one_door_safe_all_doors_safe with (d' := d) in safe;
-    case: postc=>[postc ->] //=.
+case=> d x prec postc safe; apply one_door_safe_all_doors_safe with (d := d);
+  apply one_door_safe_all_doors_safe with (d' := d) in safe;
+  case: postc=> [postc ->] //=.
 
-  case: safe=> [left_safe|right_safe]; right; rewrite tog_equ_2 //=.
-  exact: doors_toggle_callerE.
+case: safe=> [left_safe | right_safe]; right; rewrite tog_equ_2 //=.
+exact: doors_toggle_callerE.
 Qed.
 
 Lemma respectful_run_inv `{Provide ix DOORS} {A} (p : freer ix A)
     (ω : Ω) (safe : sel left ω = false \/ sel right ω = false)
     (a : A) (ω' : Ω)
     (hpre : pre (to_hoare
-      (im:=Freer.Monad_acto__canonical__Impure_MonadFreer ix)
+      (im:=freer ix)
       doors_contract p) ω)
     (hpost : post (to_hoare
-      (im:=Freer.Monad_acto__canonical__Impure_MonadFreer ix)
+      (im:=freer ix)
       doors_contract p) ω a ω') :
   sel left ω' = false \/ sel right ω' = false.
-
 (** We reason by induction on the impure computation [p]:
 
     - Either [p] is a local, pure computation; in such a case, the doors state
       does not change, hence the proof is trivial.
 
-    - Or [p] consists in a request to the doors interface, and a continuation
+    - Or [p] consists in a request to the doors effect, and a continuation
       whose domain satisfies the theorem, i.e. it preserves the invariant that
       either the left or the right door is closed.  Due to this hypothesis, we
       only have to prove that the first request made by [p] does not break the
@@ -454,7 +387,7 @@ Proof.
 rewrite -co_leftE in safe hpre hpost |-*.
 move: p ω hpre hpost safe.
 elim=> [result | b e f ih] ω + + safe.
-  rewrite to_hoare_local_postE=>? [_ witness].
+- rewrite to_hoare_local_postE=> ? [_ witness].
   subst ω'.
   exact: safe.
 rewrite to_hoare_impure_preE to_hoare_impure_postE.
@@ -470,19 +403,18 @@ Qed.
 
 (** ** Main Theorem *)
 Definition correct_component `{MayProvide jx j}
-   `(c : component i jx) `(ci : contract i Ωi) `(cj : contract j Ωj)
-    (pred : Ωi -> Ωj -> Prop)
-  : Prop :=
-   forall (ωi : Ωi) (ωj : Ωj) (init : pred ωi ωj)
-         `(e : i α) (o_caller : caller_obligation ci ωi e),
+    `(c : component i jx) `(ci : contract i Ωi) `(cj : contract j Ωj)
+    (pred : Ωi -> Ωj -> Prop) :
+  Prop :=
+  forall (ωi : Ωi) (ωj : Ωj) (init : pred ωi ωj)
+      `(e : i α) (o_caller : caller_obligation ci ωi e),
     pre (to_hoare cj $ c α e) ωj /\
     forall (x : α) (ωj' : Ωj),
       post (to_hoare
-        (im:=Freer.Monad_acto__canonical__Impure_MonadFreer jx)
+        (im:=freer jx)
         cj (c α e)) ωj x ωj' ->
       callee_obligation ci ωi e x /\
       pred (witness_update ci ωi e x) ωj'.
-
 
 Lemma gen_witness_update_otherE
     `{Provide ix i, MayProvide ix j, Distinguish ix i j}
@@ -490,29 +422,29 @@ Lemma gen_witness_update_otherE
   gen_witness_update c ω (inj_p e) x = ω.
 Proof. by rewrite /gen_witness_update distinguish. Qed.
 
-
 Lemma controller_correct `{StrictProvide2 ix DOORS (STORE nat)}
   : correct_component controller
-                      (no_contract CONTROLLER)
-                      doors_contract
-                      (fun _ ω => sel left ω = false \/ sel right ω = false).
+    (no_contract CONTROLLER)
+    doors_contract
+    (fun _ ω => sel left ω = false \/ sel right ω = false).
 Proof.
 move=> ωc ωd safe A eff _.
 (* clear request_ok. *)
 have hpre :
-    pre (to_hoare
-           (im:=Freer.Monad_acto__canonical__Impure_MonadFreer ix)
-           doors_contract (controller A eff)) ωd.
+  pre (to_hoare
+    (im:=freer ix)
+    doors_contract (controller A eff)) ωd.
 case: eff => [|d]; rewrite /controller/iget.
 - apply: to_hoare_bind_preI.
   + exact: store_request_preI.
   + move=> x om /to_hoare_request_postE [_ +].
-    rewrite (gen_witness_update_otherE (ix:=ix) (i:=STORE nat) (j:=DOORS))=> ->.
+    rewrite (gen_witness_update_otherE (ix:=ix) (i:=STORE nat)
+      (j:=DOORS))=> ->.
     case: (15 <? x) => //=.
     apply: to_hoare_bind_preI=> //.
     apply: to_hoare_bind_preI.
-      * by apply: to_hoare_bind_preI=> [|???]; exact/close_door_respectful.
-      * by move=> ???; exact: store_request_preI.
+    * by apply: to_hoare_bind_preI=> [|???]; exact/close_door_respectful.
+    * by move=> ???; exact: store_request_preI.
 - apply: to_hoare_bind_preI.
   + apply: to_hoare_bind_preI.
     * exact: close_door_respectful.
@@ -523,4 +455,4 @@ split=> //?? run; split=> //.
 exact: respectful_run_inv _ _ safe _ _ hpre run.
 Qed.
 
-End a.
+End airlock_s.
