theories/HoareFacts.v
@@ -38,12 +38,12 @@ Lemma to_hoare_local_preE `(x : a) (ω : Ω) : pre (to_hoare c (pure x)) ω.
 Proof. by rewrite to_hoare_localE hoare_pure_preE. Qed.
 
 Lemma to_hoare_bindE `(p : freer ix a) `(f : a -> freer ix b) :
-  to_hoare c (freer_bind p f) =
+  to_hoare c (p >>= f) =
   to_hoare c p >>= fun x => to_hoare c (f x).
 Proof. exact: denote_bind. Qed.
 
 Lemma to_hoare_bind_preE `(p : freer ix a) `(f : a -> freer ix b) (ω : Ω) :
-  pre (to_hoare c (freer_bind p f)) ω <->
+  pre (to_hoare c (p >>= f)) ω <->
   pre (to_hoare c p) ω /\
   forall x ω',
     post (to_hoare c p) ω x ω' -> pre (to_hoare c (f x)) ω'.
@@ -54,7 +54,7 @@ Lemma to_hoare_bind_preI `(p : freer ix a) `(f : a -> freer ix b) (ω : Ω) :
   (forall x ω',
     post (to_hoare c p) ω x ω' ->
     pre (to_hoare c (f x)) ω') ->
-  pre (to_hoare c (freer_bind p f)) ω.
+  pre (to_hoare c (p >>= f)) ω.
 Proof. by move=> prefix suffix; apply/to_hoare_bind_preE; split. Qed.
 
 End tmp.
@@ -86,14 +86,16 @@ Proof. by rewrite to_hoare_requestE; exact: interface_to_hoare_postI. Qed.
 Lemma to_hoare_local_preI `(x : a) (ω : Ω) : pre (to_hoare c (pure x)) ω.
 Proof. by apply/to_hoare_local_preE. Qed.
 
+Lemma to_hoare_skip_preI (ω : Ω) :
+  pre (to_hoare c (skip : freer ix unit)) ω.
+Proof. exact: to_hoare_local_preI. Qed.
+
 Lemma to_hoare_local_postE `(x : a) (y : a) (ω ω' : Ω) :
-  post (to_hoare c (pure x : freer ix a)) ω y ω' <->
-  x = y /\ ω = ω'.
+  post (to_hoare c (pure x)) ω y ω' <-> x = y /\ ω = ω'.
 Proof. by rewrite to_hoare_localE hoare_pure_postE. Qed.
 
 Lemma to_hoare_local_postI `(x : a) (ω : Ω) :
-  post (to_hoare (im:=Freer.Monad_acto__canonical__Impure_MonadFreer ix)
-                 c (pure x : freer ix a)) ω x ω.
+  post (to_hoare c (pure x)) ω x ω.
 Proof. by apply/to_hoare_local_postE; split. Qed.
 
 End tmp.
@@ -105,155 +107,87 @@ Context `{MayProvide ix i} `(c : contract i Ω)
     `(p : freer ix a) `(f : a -> freer ix b).
 
 Lemma to_hoare_bind_postE (ω : Ω) (y : b) (ω' : Ω) :
-  post (to_hoare (im:=Freer.Monad_acto__canonical__Impure_MonadFreer ix)
-                 c (freer_bind p f)) ω y ω' <->
+  post (to_hoare c (p >>= f)) ω y ω' <->
   exists x ω'',
-    post (to_hoare
-            (im:=Freer.Monad_acto__canonical__Impure_MonadFreer ix)
-            c p) ω x ω'' /\
-    post (to_hoare
-            (im:=Freer.Monad_acto__canonical__Impure_MonadFreer ix)
-            c (f x)) ω'' y ω'.
+    post (to_hoare c p) ω x ω'' /\ post (to_hoare c (f x)) ω'' y ω'.
 Proof. by rewrite to_hoare_bindE hoare_bind_postE. Qed.
 
 Lemma to_hoare_bind_postI
     (ω : Ω) (x : a) (ω'' : Ω) (y : b) (ω' : Ω) :
-  post (to_hoare (im:=Freer.Monad_acto__canonical__Impure_MonadFreer ix)
-                 c p) ω x ω'' ->
-  post (to_hoare (im:=Freer.Monad_acto__canonical__Impure_MonadFreer ix)
-                 c (f x)) ω'' y ω' ->
-  post (to_hoare (im:=Freer.Monad_acto__canonical__Impure_MonadFreer ix)
-                 c (freer_bind p f)) ω y ω'.
+  post (to_hoare c p) ω x ω'' ->
+  post (to_hoare c (f x)) ω'' y ω' ->
+  post (to_hoare c (p >>= f)) ω y ω'.
 Proof.
-move=> prefix suffix; apply/to_hoare_bind_postE.
-by exists x, ω''.
+by move=> prefix suffix; apply/to_hoare_bind_postE; exists x, ω''.
 Qed.
 
 End tmp.
 
 Lemma to_hoare_impure_preE `{MayProvide ix i} `(c : contract i Ω)
     `(e : ix a) `(f : a -> freer ix b) (ω : Ω) :
-  pre (to_hoare (im:=Freer.Monad_acto__canonical__Impure_MonadFreer ix)
-                c (impure e f)) ω <->
-  gen_caller_obligation c ω e /\
-  forall x, gen_callee_obligation c ω e x ->
-    pre (to_hoare (im:=Freer.Monad_acto__canonical__Impure_MonadFreer ix)
-                  c (f x)) (gen_witness_update c ω e x).
+  pre (to_hoare c (impure e f)) ω <->
+  gen_caller_obligation c ω e /\ forall x, gen_callee_obligation c ω e x ->
+    pre (to_hoare c (f x)) (gen_witness_update c ω e x).
 Proof.
-change
-  (pre (interface_to_hoare c e >>=
-          fun x =>
-            to_hoare
-              (im:=Freer.Monad_acto__canonical__Impure_MonadFreer ix)
-              c (f x)) ω <->
-   gen_caller_obligation c ω e /\
-   forall x, gen_callee_obligation c ω e x ->
-     pre (to_hoare
-            (im:=Freer.Monad_acto__canonical__Impure_MonadFreer ix)
-            c (f x)) (gen_witness_update c ω e x)).
 split.
 - move=> /hoare_bind_preE [caller next]; split.
-    exact/interface_to_hoare_preE.
-  move=> x callee; apply: next.
-  exact/interface_to_hoare_postI.
-move=> [caller next]; apply/hoare_bind_preE; split.
-  exact/interface_to_hoare_preE.
-move=> x ω' /interface_to_hoare_postE [callee ->].
-exact: next.
+  + exact/interface_to_hoare_preE.
+  + by move=> x callee; apply: next; exact/interface_to_hoare_postI.
+- move=> [caller next]; apply/hoare_bind_preE; split.
+  + exact/interface_to_hoare_preE.
+  + by move=> x ω' /interface_to_hoare_postE [callee ->]; exact: next.
 Qed.
 
 Lemma to_hoare_impure_preI `{MayProvide ix i} `(c : contract i Ω)
     `(e : ix a) `(f : a -> freer ix b) (ω : Ω) :
   gen_caller_obligation c ω e ->
   (forall x, gen_callee_obligation c ω e x ->
-    pre (to_hoare (im:=Freer.Monad_acto__canonical__Impure_MonadFreer ix)
-                  c (f x)) (gen_witness_update c ω e x)) ->
-  pre (to_hoare (im:=Freer.Monad_acto__canonical__Impure_MonadFreer ix)
-                c (impure e f)) ω.
+    pre (to_hoare c (f x)) (gen_witness_update c ω e x)) ->
+  pre (to_hoare c (impure e f)) ω.
 Proof. by move=> caller next; apply/to_hoare_impure_preE; split. Qed.
 
 Lemma to_hoare_impure_postE `{MayProvide ix i} `(c : contract i Ω)
     `(e : ix a) `(f : a -> freer ix b) (ω : Ω) (y : b) (ω' : Ω) :
-  post (to_hoare (im:=Freer.Monad_acto__canonical__Impure_MonadFreer ix)
-                 c (impure e f)) ω y ω' <->
+  post (to_hoare c (impure e f)) ω y ω' <->
   exists x, gen_callee_obligation c ω e x /\
-    post (to_hoare (im:=Freer.Monad_acto__canonical__Impure_MonadFreer ix)
-                   c (f x)) (gen_witness_update c ω e x) y ω'.
+    post (to_hoare c (f x)) (gen_witness_update c ω e x) y ω'.
 Proof.
-change
-  (post (interface_to_hoare c e >>=
-           fun x =>
-             to_hoare
-               (im:=Freer.Monad_acto__canonical__Impure_MonadFreer ix)
-               c (f x)) ω y ω' <->
-   exists x, gen_callee_obligation c ω e x /\
-     post (to_hoare
-             (im:=Freer.Monad_acto__canonical__Impure_MonadFreer ix)
-             c (f x)) (gen_witness_update c ω e x) y ω').
 split.
-- move=> /hoare_bind_postE [x [ω'' [step suffix]]].
-  move: step => /interface_to_hoare_postE [callee witness].
-  subst ω''.
-  by exists x.
-move=> [x [callee suffix]]; apply/hoare_bind_postE.
-exists x, (gen_witness_update c ω e x); split=> //.
+- move=> /hoare_bind_postE [x [ω'' [+ suffix]]].
+  rewrite interface_to_hoare_postE.
+  by move=> [callee witness]; subst ω''; exists x.
+- move=> [x [callee suffix]]; apply/hoare_bind_postE.
+  by exists x, (gen_witness_update c ω e x); split.
 Qed.
 
 (** * General Lemmas *)
 
 Lemma to_hoare_step `{MayProvide ix i} `(c : contract i Ω)
     `(e : ix a) `(f : a -> freer ix a)
-    `(hpre : pre (to_hoare
-      (im:=Freer.Monad_acto__canonical__Impure_MonadFreer ix)
-      c (impure e f)) ω)
+    `(hpre : pre (to_hoare c (impure e f)) ω)
     (x : a) (step : gen_callee_obligation c ω e x) :
-  pre (to_hoare
-         (im:=Freer.Monad_acto__canonical__Impure_MonadFreer ix)
-         c (f x)) (gen_witness_update c ω e x).
-
-Proof.
-move: hpre => /to_hoare_impure_preE [_ next].
-exact: next.
-Qed.
+  pre (to_hoare c (f x)) (gen_witness_update c ω e x).
+Proof. by move: hpre => /to_hoare_impure_preE [_ +]; exact. Qed.
 
 #[global] Hint Resolve to_hoare_step : freespec.
 
 Lemma to_hoare_pre_bind_assoc `{MayProvide ix i} `(c : contract i Ω)
     `(p : freer ix a)
-    `(Hp : pre (to_hoare
-      (im:=Freer.Monad_acto__canonical__Impure_MonadFreer ix) c p) ω)
+    `(Hp : pre (to_hoare c p) ω)
     `(f : a -> freer ix b)
     (run : forall (x : a) (ω' : Ω),
-      post (to_hoare
-        (im:=Freer.Monad_acto__canonical__Impure_MonadFreer ix)
-        c p) ω x ω' ->
-      pre (to_hoare
-        (im:=Freer.Monad_acto__canonical__Impure_MonadFreer ix)
-        c (f x)) ω') :
-  pre (to_hoare
-         (im:=Freer.Monad_acto__canonical__Impure_MonadFreer ix)
-         c (freer_bind p f)) ω.
-
-Proof.
-by apply/to_hoare_bind_preI.
-Qed.
+      post (to_hoare c p) ω x ω' ->
+      pre (to_hoare c (f x)) ω') :
+  pre (to_hoare c (p >>= f)) ω.
+Proof. exact/to_hoare_bind_preI. Qed.
 
 Lemma to_hoare_post_bind_assoc `{MayProvide ix i} `(c : contract i Ω)
     `(p : freer ix a) `(f : a -> freer ix b)
-    `(Hp : post (to_hoare
-      (im:=Freer.Monad_acto__canonical__Impure_MonadFreer ix)
-      c (freer_bind p f)) ω x ω') :
+    `(Hp : post (to_hoare c (p >>= f)) ω x ω') :
   exists y ω'',
-    post (to_hoare
-      (im:=Freer.Monad_acto__canonical__Impure_MonadFreer ix)
-      c p) ω y ω'' /\
-    post (to_hoare
-      (im:=Freer.Monad_acto__canonical__Impure_MonadFreer ix)
-      c (f y)) ω'' x ω'.
-
-Proof.
-exact/to_hoare_bind_postE.
-Qed.
+    post (to_hoare c p) ω y ω'' /\
+    post (to_hoare c (f y)) ω'' x ω'.
+Proof. exact/to_hoare_bind_postE. Qed.
 
 (** * Contract Product Views *)
 
@@ -282,18 +216,15 @@ Proof. by []. Qed.
 Lemma to_hoare_contractprod_preI `{Provide ix i, Provide ix j}
     `(ci : contract i Ωi) `(cj : contract j Ωj)
     `(p : freer ix a) (ωi : Ωi) (ωj : Ωj) :
-  pre (to_hoare (im:=Freer.Monad_acto__canonical__Impure_MonadFreer ix)
-                ci p) ωi ->
-  pre (to_hoare (im:=Freer.Monad_acto__canonical__Impure_MonadFreer ix)
-                cj p) ωj ->
-  pre (to_hoare (im:=Freer.Monad_acto__canonical__Impure_MonadFreer ix)
-                (ci * cj) p) (ωi, ωj).
+  pre (to_hoare ci p) ωi ->
+  pre (to_hoare cj p) ωj ->
+  pre (to_hoare (ci * cj) p) (ωi, ωj).
 Proof.
 move: p ωi ωj.
 elim=> [x | b e f ih] ωi ωj.
-- by move=> _ _; apply/to_hoare_local_preE.
-move=> /to_hoare_impure_preE [calleri nexti].
-move=> /to_hoare_impure_preE [callerj nextj].
+  by move=> _ _; apply/to_hoare_local_preE.
+rewrite 2!to_hoare_impure_preE.
+move=> [calleri nexti] [callerj nextj].
 apply/to_hoare_impure_preI.
   by apply/contractprod_callerE; split.
 move=> x /contractprod_calleeE [calleei calleej].
@@ -305,39 +236,31 @@ Qed.
 
 Lemma to_hoare_contractprod `{Provide ix i, Provide ix j}
     `(ci : contract i Ωi) `(cj : contract j Ωj)
-    `(p : freer ix a) `(prei : pre (to_hoare
-      (im:=Freer.Monad_acto__canonical__Impure_MonadFreer ix) ci p) ωi)
-    `(prej : pre (to_hoare
-      (im:=Freer.Monad_acto__canonical__Impure_MonadFreer ix) cj p) ωj) :
-  pre (to_hoare (im:=Freer.Monad_acto__canonical__Impure_MonadFreer ix)
-                (ci * cj) p) (ωi, ωj).
+    `(p : freer ix a) `(prei : pre (to_hoare ci p) ωi)
+    `(prej : pre (to_hoare cj p) ωj) :
+  pre (to_hoare (ci * cj) p) (ωi, ωj).
 Proof. exact: to_hoare_contractprod_preI prei prej. Qed.
 
 #[global] Hint Resolve to_hoare_contractprod_preI : freespec.
 
 Lemma contract_equ_pre `(c1 : contract i Ω1) `(c2 : contract i Ω2)
     `(equ : contract_equ c1 c2) (ω1 : Ω1) `(p : freer i A) :
-  pre (to_hoare
-         (im:=Freer.Monad_acto__canonical__Impure_MonadFreer i)
-         c1 p) ω1 <->
-  pre (to_hoare
-         (im:=Freer.Monad_acto__canonical__Impure_MonadFreer i)
-         c2 p) (contract_iso_lr equ ω1).
-
+  pre (to_hoare c1 p) ω1 <->
+  pre (to_hoare c2 p) (contract_iso_lr equ ω1).
 Proof.
-  elim: equ => f g iso1 iso2 caller_equ callee_equ witness_equ.
-  move: ω1.
-  elim: p=> [a | B e k IH] ω1. 
-  - by split.
-  rewrite /= /gen_caller_obligation /gen_callee_obligation
-              /gen_witness_update /=.
-  rewrite (caller_equ ω1 B e).
-  setoid_rewrite (callee_equ ω1 B e).
-  split => [[ocaller onext] | [ocaller onext]];
+elim: equ => f g iso1 iso2 caller_equ callee_equ witness_equ.
+move: ω1.
+elim: p=> [a | B e k IH] ω1.
+- by split.
+rewrite /= /gen_caller_obligation /gen_callee_obligation
+  /gen_witness_update /=.
+rewrite (caller_equ ω1 B e).
+setoid_rewrite (callee_equ ω1 B e).
+split => [[ocaller onext] | [ocaller onext]];
   split => // x ω1' [ocallee owitness].
-  - by rewrite owitness -witness_equ -IH; eauto.
-  rewrite IH; eauto.
-  rewrite owitness /= witness_equ; eauto.
+- by rewrite owitness -witness_equ -IH; eauto.
+rewrite IH; eauto.
+rewrite owitness /= witness_equ; eauto.
 Qed.
 
 #[global] Hint Resolve contract_equ_pre : freespec.
@@ -345,23 +268,18 @@ Qed.
 Lemma contract_equ_post `(c1 : contract i Ω1) `(c2 : contract i Ω2)
     `(equ : contract_equ c1 c2) (ω1 ω1' : Ω1)
     `(p : freer i A) (x : A)
-    (post1 : post (to_hoare
-      (im:=Freer.Monad_acto__canonical__Impure_MonadFreer i)
-      c1 p) ω1 x ω1') :
-  post (to_hoare
-          (im:=Freer.Monad_acto__canonical__Impure_MonadFreer i)
-          c2 p) (contract_iso_lr equ ω1) x
+    (post1 : post (to_hoare c1 p) ω1 x ω1') :
+  post (to_hoare c2 p) (contract_iso_lr equ ω1) x
        (contract_iso_lr equ ω1').
-
 Proof.
-  elim:equ=> [f g iso1 iso2 caller_equ callee_equ witness_equ].
-  move: p x ω1 ω1' post1.
-  elim=>[in_a | B e k IH]=> a ω1 ω1' [b witness] /=.
-  + by subst a; subst ω1'; split.
-  + move: witness=> [ω1'' [[ocallee owitness] +]] /= => /IH post1.
-    exists b, (f ω1''); split; [split|exact: post1].
-    * exact/(callee_equ ω1 B e).
-    * by rewrite owitness witness_equ.
+elim: equ => [f g iso1 iso2 caller_equ callee_equ witness_equ].
+move: p x ω1 ω1' post1.
+elim=> [in_a | B e k IH]=> a ω1 ω1' [b witness] /=.
+- by subst a; subst ω1'; split.
+- move: witness=> [ω1'' [[ocallee owitness] +]] /= => /IH post1.
+  exists b, (f ω1''); split; [split|exact: post1].
+  + exact/(callee_equ ω1 B e).
+  + by rewrite owitness witness_equ.
 Qed.
 
 #[global] Hint Resolve contract_equ_post : freespec.
